Add memory wellformedness and mstore disambiguation, admit proofs (#17)

src/Memory.ec
@@ -2,3 +2,13 @@ require import UInt256.
 require export CoreMap SmtMap.
 
 type mem = (uint256, uint256) map.
+pred mem_wellformed (memory: mem) = forall (idx: uint256), memory.[idx] <= W256.masklsb 8.
+
+lemma write_byte_maintains_wellformed (memory: mem) (idx val: uint256):
+    val < W256.masklsb 8 =>
+    mem_wellformed memory =>
+    mem_wellformed (memory.[idx <- val]).
+    proof.
+      progress.
+      smt ().
+    qed.
